Merge work done so far on composition.
A notable related change regards the defintion of the complete
intermediate semantics. I introduced our specific state equality because
of the presence of Coq's maps in our states. This was needed when I was
trying to make stepping a state which was built by merging partial states.

Intermediate/CS.v
@@ -16,7 +16,7 @@ Definition stack : Type := list Pointer.t.
 
 Definition state : Type := stack * Memory.t * Register.t * Pointer.t.
 
-Ltac unfold_state :=
+Ltac unfold_states :=
   match goal with
   | H: state |- _ =>
     let s := fresh "s" in
@@ -39,7 +39,7 @@ Lemma state_eq_refl:
     state_eq s s.
 Proof.
   intros s.
-  unfold_state.
+  unfold_states.
   constructor; reflexivity.
 Qed.
 
@@ -79,25 +79,20 @@ Instance state_turn : HasTurn state := {
 
 (* transition system *)
 
-Definition initial_state (p: program) (s: state) : Prop :=
-  let G := init_genv p in
-  let '(gps, mem, regs, pc) := s in
-
-  (* the global protected stack is empty *)
-  gps = [] /\
-
-  (* mem exactly contains all components memories and it comes from the init routine *)
-  (forall C, PMap.In C (prog_interface p) <-> PMap.In C mem) /\
-  (let '(m, _, _) := init_all p in mem = m) /\
-
-  (* the registers are set to undef *)
-  regs = [Undef; Undef; Undef; Undef; Undef; Undef] /\
-
-  (* the program counter is pointing to the start of the main procedure *)
-  Pointer.component pc = fst (prog_main p) /\
-  EntryPoint.get (fst (prog_main p)) (snd (prog_main p))
-                 (genv_entrypoints G) = Some (Pointer.block pc) /\
-  Pointer.offset pc = 0.
+Inductive initial_state (p: program): state -> Prop :=
+| initial_state_intro: forall gps mem regs pc,
+    (* the global protected stack is empty *)
+    gps = [] ->
+    (* mem comes from the init routine *)
+    PMap.Equal mem (let '(m, _, _) := init_all p in m) ->
+    (* the registers are set to undef *)
+    regs = [Undef; Undef; Undef; Undef; Undef; Undef] ->
+    (* the program counter is pointing to the start of the main procedure *)
+    Pointer.component pc = fst (prog_main p) ->
+    EntryPoint.get (fst (prog_main p)) (snd (prog_main p))
+                   (genv_entrypoints (init_genv p)) = Some (Pointer.block pc) ->
+    Pointer.offset pc = 0 ->
+    initial_state p (gps, mem, regs, pc).
 
 Definition final_state (G: global_env) (s: state) : Prop :=
   let '(gsp, mem, regs, pc) := s in
@@ -106,193 +101,244 @@ Definition final_state (G: global_env) (s: state) : Prop :=
 (* relational specification *)
 
 Inductive step (G : global_env) : state -> trace -> state -> Prop :=
-| Nop: forall gps mem regs pc,
+| Nop: forall ics ics' gps mem regs pc,
+    state_eq ics (gps, mem, regs, pc) ->
     executing G pc INop ->
-    step G (gps, mem, regs, pc) E0 (gps, mem, regs, Pointer.inc pc)
+    state_eq ics' (gps, mem, regs, Pointer.inc pc) ->
+    step G ics E0 ics'
 
-| Label: forall gps mem regs pc l,
+| Label: forall ics ics' gps mem regs pc l,
+    state_eq ics (gps, mem, regs, pc) ->
     executing G pc (ILabel l) ->
-    step G (gps, mem, regs, pc) E0 (gps, mem, regs, Pointer.inc pc)
+    state_eq ics' (gps, mem, regs, Pointer.inc pc) ->
+    step G ics E0 ics'
 
-| Const: forall gps mem regs regs' pc r v,
+| Const: forall ics ics' gps mem regs regs' pc r v,
+    state_eq ics (gps, mem, regs, pc) ->
     executing G pc (IConst v r) ->
     Register.set r (imm_to_val v) regs = regs' ->
-    step G (gps, mem, regs, pc) E0 (gps, mem, regs', Pointer.inc pc)
+    state_eq ics' (gps, mem, regs', Pointer.inc pc) ->
+    step G ics E0 ics'
 
-| Mov: forall gps mem regs regs' pc r1 r2,
+| Mov: forall ics ics' gps mem regs regs' pc r1 r2,
+    state_eq ics (gps, mem, regs, pc) ->
     executing G pc (IMov r1 r2) ->
     Register.set r2 (Register.get r1 regs) regs = regs' ->
-    step G (gps, mem, regs, pc) E0 (gps, mem, regs', Pointer.inc pc)
+    state_eq ics' (gps, mem, regs', Pointer.inc pc) ->
+    step G ics E0 ics'
 
-| BinOp: forall gps mem regs regs' pc r1 r2 r3 op,
+| BinOp: forall ics ics' gps mem regs regs' pc r1 r2 r3 op,
+    state_eq ics (gps, mem, regs, pc) ->
     executing G pc (IBinOp op r1 r2 r3) ->
-    Register.set r3
-                 (eval_binop op (Register.get r1 regs) (Register.get r2 regs))
-                 regs = regs' ->
-    step G (gps, mem, regs, pc) E0 (gps, mem, regs', Pointer.inc pc)
+    let result := eval_binop op (Register.get r1 regs) (Register.get r2 regs) in
+    Register.set r3 result regs = regs' ->
+    state_eq ics' (gps, mem, regs', Pointer.inc pc) ->
+    step G ics E0 ics'
 
-| Load: forall gps mem regs regs' pc r1 r2 ptr v,
+| Load: forall ics ics' gps mem regs regs' pc r1 r2 ptr v,
+    state_eq ics (gps, mem, regs, pc) ->
     executing G pc (ILoad r1 r2) ->
     Register.get r1 regs = Ptr ptr ->
     Pointer.component ptr = Pointer.component pc ->
     Memory.load mem ptr = Some v ->
     Register.set r2 v regs = regs' ->
-    step G (gps, mem, regs, pc) E0 (gps, mem, regs', Pointer.inc pc)
+    state_eq ics' (gps, mem, regs', Pointer.inc pc) ->
+    step G ics E0 ics'
 
-| Store: forall gps mem regs pc ptr r1 r2 mem',
+| Store: forall ics ics' gps mem mem' regs pc ptr r1 r2,
+    state_eq ics (gps, mem, regs, pc) ->
     executing G pc (IStore r1 r2) ->
     Register.get r1 regs = Ptr ptr ->
     Pointer.component ptr = Pointer.component pc ->
     Memory.store mem ptr (Register.get r2 regs) = Some mem' ->
-    step G (gps, mem, regs, pc) E0 (gps, mem', regs, Pointer.inc pc)
+    state_eq ics' (gps, mem', regs, Pointer.inc pc) ->
+    step G ics E0 ics'
 
-| Jal: forall gps mem regs regs' pc pc' l,
+| Jal: forall ics ics' gps mem regs regs' pc pc' l,
+    state_eq ics (gps, mem, regs, pc) ->
     executing G pc (IJal l) ->
     find_label_in_component G pc l = Some pc' ->
     Register.set R_RA (Ptr (Pointer.inc pc)) regs = regs' ->
-    step G (gps, mem, regs, pc) E0 (gps, mem, regs', pc')
+    state_eq ics' (gps, mem, regs', pc') ->
+    step G ics E0 ics'
 
-| Jump: forall gps mem regs pc pc' r,
+| Jump: forall ics ics' gps mem regs pc pc' r,
+    state_eq ics (gps, mem, regs, pc) ->
     executing G pc (IJump r) ->
     Register.get r regs = Ptr pc' ->
     Pointer.component pc' = Pointer.component pc ->
-    step G (gps, mem, regs, pc) E0 (gps, mem, regs, pc')
+    state_eq ics' (gps, mem, regs, pc') ->
+    step G ics E0 ics'
 
-| BnzNZ: forall gps mem regs pc pc' r l val,
+| BnzNZ: forall ics ics' gps mem regs pc pc' r l val,
+    state_eq ics (gps, mem, regs, pc) ->
     executing G pc (IBnz r l) ->
     Register.get r regs = Int val ->
     val <> 0 ->
     find_label_in_procedure G pc l = Some pc' ->
-    step G (gps, mem, regs, pc) E0 (gps, mem, regs, pc')
+    state_eq ics' (gps, mem, regs, pc') ->
+    step G ics E0 ics'
 
-| BnzZ: forall gps mem regs pc r l,
+| BnzZ: forall ics ics' gps mem regs pc r l,
+    state_eq ics (gps, mem, regs, pc) ->
     executing G pc (IBnz r l) ->
     Register.get r regs = Int 0 ->
-    step G (gps, mem, regs, pc) E0 (gps, mem, regs, Pointer.inc pc)
+    state_eq ics' (gps, mem, regs, Pointer.inc pc) ->
+    step G ics E0 ics'
 
-| Alloc: forall gps mem mem' regs regs' pc rsize rptr size ptr,
+| Alloc: forall ics ics' gps mem mem' regs regs' pc rsize rptr size ptr,
+    state_eq ics (gps, mem, regs, pc) ->
     executing G pc (IAlloc rptr rsize) ->
     Register.get rsize regs = Int size ->
-    size >= 0 ->
+    size > 0 ->
     Memory.alloc mem (Pointer.component pc) (Z.to_nat size) = Some (mem', ptr) ->
     Register.set rptr (Ptr ptr) regs = regs' ->
-    step G (gps, mem, regs, pc) E0 (gps, mem', regs', Pointer.inc pc)
+    state_eq ics' (gps, mem', regs', Pointer.inc pc) ->
+    step G ics E0 ics'
 
-| Call: forall gps gps' mem regs pc b C' P rcomval,
+| Call: forall ics ics' gps mem regs pc b C' P rcomval,
+    state_eq ics (gps, mem, regs, pc) ->
     executing G pc (ICall C' P) ->
     Pointer.component pc <> C' ->
     imported_procedure (genv_interface G) (Pointer.component pc) C' P ->
-    gps' = Pointer.inc pc :: gps ->
     EntryPoint.get C' P (genv_entrypoints G) = Some b ->
-    let pc' := (C', b, 0) in
     Register.get R_COM regs = Int rcomval ->
-    let t := [ECall (Pointer.component pc) P rcomval C'] in
-    step G (gps, mem, regs, pc) t (gps', mem, Register.invalidate regs, pc')
+    state_eq ics' (Pointer.inc pc :: gps, mem, Register.invalidate regs, (C', b, 0)) ->
+    step G ics [ECall (Pointer.component pc) P rcomval C'] ics'
 
-| Return: forall gps gps' mem regs pc pc' rcomval,
+| Return: forall ics ics' gps' mem regs pc pc' rcomval,
+    state_eq ics (pc' :: gps', mem, regs, pc) ->
     executing G pc IReturn ->
-    gps = pc' :: gps' ->
     Pointer.component pc <> Pointer.component pc' ->
     Register.get R_COM regs = Int rcomval ->
-    let t := [ERet (Pointer.component pc) rcomval (Pointer.component pc')] in
-    step G (gps, mem, regs, pc) t (gps', mem, Register.invalidate regs, pc').
+    state_eq ics' (gps', mem, Register.invalidate regs, pc') ->
+    step G ics [ERet (Pointer.component pc) rcomval (Pointer.component pc')] ics'.
 
 Lemma equal_states_step:
-  forall G ics1 t ics1' ics2,
-    state_eq ics1 ics2 ->
+  forall G ics1 t ics1' ics2 ics2',
     step G ics1 t ics1' ->
-  exists ics2',
-    step G ics2 t ics2' /\ state_eq ics1' ics2'.
+    state_eq ics1 ics2 ->
+    state_eq ics1' ics2' ->
+    step G ics2 t ics2'.
 Proof.
-  intros G ics1 t ics1' ics2.
-  intros Heq Hstep.
-  repeat CS.unfold_state.
+  intros G ics1 t ics1' ics2 ics2'.
+  intros Hstep Heq1 Heq2.
+  inversion Heq1; subst; inversion Heq2; subst.
   inversion Hstep; subst;
-  inversion Heq; subst.
+    match goal with
+    | Heq1': state_eq _ _,
+      Heq2': state_eq _ _ |- _ =>
+      inversion Heq1'; subst; inversion Heq2'; subst
+    end.
 
-  - eexists. split.
-    + eapply Nop; auto.
-    + econstructor; auto.
+  Ltac solve_mem_equality :=
+    match goal with
+    | H1: PMap.Equal ?MEM0 ?MEM1,
+      H2: PMap.Equal ?MEM0 ?MEM2,
+      H3: PMap.Equal ?MEM1 ?MEM3 |- PMap.Equal ?MEM2 ?MEM3 =>
+      rewrite H1 in H2; rewrite H2 in H3; apply H3
+    end.
 
-  - eexists. split.
-    + eapply Label; eauto.
-    + econstructor; eauto.
-
-  - eexists. split.
-    + eapply Const; eauto.
-    + econstructor; eauto.
-
-  - eexists. split.
-    + eapply Mov; eauto.
-    + econstructor; eauto.
-
-  - eexists. split.
-    + eapply BinOp; eauto.
-    + econstructor; eauto.
-
-  - eexists. split.
-    + eapply Load; eauto.
-      unfold Memory.load in * .
-      destruct ptr. destruct p.
-      rewrite H12 in H11.
-      destruct (PMap.find (elt:=ComponentMemory.t) i mem);
-        try discriminate.
+  - eapply Nop;
+      try solve_mem_equality;
       eauto.
-    + econstructor; eauto.
+    + constructor; try reflexivity.
+    + constructor; try reflexivity.
+      rewrite <- H0, <- H1, H13, H14. reflexivity.
 
-  - unfold Memory.store in * .
-    destruct ptr. destruct p.
-    rewrite H12 in H11.
-    destruct (PMap.find (elt:=ComponentMemory.t) i mem) eqn:Hfind;
-      try discriminate.
-    destruct (ComponentMemory.store t i0 o (Register.get r2 regs)) eqn:Hstore;
-      try discriminate.
-    inversion H11. subst.
-    eexists. split.
-    + eapply Store; eauto.
-      unfold Memory.store in *.
-      rewrite Hfind, Hstore. eauto.
-    + econstructor; eauto.
-      rewrite H12. reflexivity.
+  - eapply Label;
+      try solve_mem_equality;
+      eauto.
+    + constructor; try reflexivity.
+    + constructor; try reflexivity.
+      rewrite <- H0, <- H1, H13, H14. reflexivity.
 
-  - eexists. split.
-    + eapply Jal; eauto.
-    + econstructor; eauto.
+  - eapply Const;
+      try solve_mem_equality;
+      eauto.
+    + constructor; try reflexivity.
+    + constructor; try reflexivity.
+      rewrite <- H0, <- H1, H13, H14. reflexivity.
 
-  - eexists. split.
-    + eapply Jump; eauto.
-    + econstructor; eauto.
+  - eapply Mov;
+      try solve_mem_equality;
+      eauto.
+    + constructor; try reflexivity.
+    + constructor; try reflexivity.
+      rewrite <- H0, <- H1, H13, H14. reflexivity.
 
-   - eexists. split.
-    + eapply BnzNZ; eauto.
-    + econstructor; eauto.
+  - eapply BinOp;
+      try solve_mem_equality;
+      eauto.
+    + constructor; try reflexivity.
+    + constructor; try reflexivity.
+      rewrite <- H0, <- H1, H13, H14. reflexivity.
 
-   - eexists. split.
-    + eapply BnzZ; eauto.
-    + econstructor; eauto.
+  - eapply Load;
+      try solve_mem_equality;
+      eauto.
+    + constructor; try reflexivity.
+      rewrite <- H0. auto.
+    + constructor; try reflexivity.
+      rewrite <- H1. auto.
 
-   - unfold Memory.alloc in * .
-     destruct pc. destruct p.
-     rewrite H12 in H11. simpl in *.
-     destruct (PMap.find (elt:=ComponentMemory.t) i mem) eqn:Hfind;
-       try discriminate.
-     destruct (ComponentMemory.alloc t (Z.to_nat size)) eqn:Halloc;
-       try discriminate.
-     inversion H11. subst.
-     eexists. split.
-     + eapply Alloc; eauto.
-       unfold Memory.alloc in *.
-       simpl. rewrite Hfind, Halloc. eauto.
-     + econstructor; eauto.
-       rewrite H12. reflexivity.
+  - eapply Store;
+      try solve_mem_equality;
+      eauto.
+    + constructor; try reflexivity.
+      rewrite <- H0. auto.
+    + constructor; try reflexivity.
+      rewrite <- H1. auto.
 
-   - eexists. split.
-    + eapply Call; eauto.
-    + econstructor; eauto.
+  - eapply Jal;
+      try solve_mem_equality;
+      eauto.
+    + constructor; try reflexivity.
+    + constructor; try reflexivity.
+      rewrite <- H0, <- H1, H14, H15. reflexivity.
 
-   - eexists. split.
-    + eapply Return; eauto.
-    + econstructor; eauto.
+  - eapply Jump;
+      try solve_mem_equality;
+      eauto.
+    + constructor; try reflexivity.
+    + constructor; try reflexivity.
+      rewrite <- H0, <- H1, H15, H16. reflexivity.
+
+  - eapply BnzNZ;
+      try solve_mem_equality;
+      eauto.
+    + constructor; try reflexivity.
+    + constructor; try reflexivity.
+      rewrite <- H0, <- H1, H16, H17. reflexivity.
+
+  - eapply BnzZ;
+      try solve_mem_equality;
+      eauto.
+    + constructor; try reflexivity.
+    + constructor; try reflexivity.
+      rewrite <- H0, <- H1, H14, H15. reflexivity.
+
+  - eapply Alloc;
+      try solve_mem_equality;
+      eauto.
+    + constructor; try reflexivity.
+      rewrite <- H0. auto.
+    + constructor; try reflexivity.
+      rewrite <- H1. auto.
+
+  - eapply Call;
+      try solve_mem_equality;
+      eauto.
+    + constructor; try reflexivity.
+    + constructor; try reflexivity.
+      rewrite <- H0, <- H1, H17, H18. reflexivity.
+
+  - eapply Return;
+      try solve_mem_equality;
+      eauto.
+    + constructor; try reflexivity.
+    + constructor; try reflexivity.
+      rewrite <- H0, <- H1, H15, H16. reflexivity.
 Qed.
 
 (* executable specification *)
@@ -372,7 +418,7 @@ Definition eval_step (G: global_env) (s: state) : option (trace * state) :=
     | IAlloc rptr rsize =>
       match Register.get rsize regs with
       | Int size =>
-        if size <? 0 then
+        if size <=? 0 then
           None
         else
           do (mem', ptr) <- Memory.alloc mem (Pointer.component pc) (Z.to_nat size);
@@ -446,86 +492,177 @@ Close Scope monad_scope.
 
 Theorem eval_step_complete:
   forall G st t st',
-    step G st t st' -> eval_step G st =  Some (t, st').
+    step G st t st' ->
+  exists st'',
+    eval_step G st = Some (t, st'') /\ state_eq st' st''.
 Proof.
   intros G st t st' Hstep.
   inversion Hstep; subst;
-    destruct H as [procs [P_code [Hprocs [HP_code [? Hinstr]]]]];
+    (* extract information about the state *)
+    match goal with
+    | Hexec: executing _ _ _,
+      Heq1: state_eq _ _,
+      Heq2: state_eq _ _ |- _ =>
+      destruct Hexec as [procs [P_code [Hprocs [HP_code [? Hinstr]]]]];
+      inversion Heq1; subst; clear Heq1; inversion Heq2; subst; clear Heq2
+    end;
+    (* simplify *)
     simpl; unfold code in *; rewrite Hprocs, HP_code, Hinstr;
-    destruct (Pointer.offset pc) eqn:Hpc;
-    try reflexivity; try (exfalso; pose proof (Zlt_neg_0 p); omega).
-  - simpl. rewrite H0, H1.
-    destruct pc. destruct p. simpl.
-    rewrite Pos.eqb_refl. rewrite H2. reflexivity.
-  - rewrite H0, H1, H2. rewrite Pos.eqb_refl.
-    apply Z.ge_le_iff in H.
-    apply Z.ltb_ge in H.
-    rewrite H. reflexivity.
-  - rewrite Z.ltb_irrefl, H0, H1, H2, Pos.eqb_refl.
-    simpl. reflexivity.
-  - rewrite H0, H1, H2.
-    rewrite Pos.eqb_refl. reflexivity.
-  - simpl. rewrite H0. reflexivity.
-  - simpl. rewrite H0. reflexivity.
-  - rewrite H0, H1.
-    rewrite Pos.eqb_refl. reflexivity.
-  - rewrite H0, H1.
-    rewrite Pos.eqb_refl. reflexivity.
-  - rewrite H0, H2.
-    destruct val.
-    + contradiction.
-    + reflexivity.
-    + simpl. reflexivity.
-  - simpl. rewrite H0, H2. destruct val.
-    + contradiction.
-    + reflexivity.
-    + reflexivity.
-  - rewrite H0. reflexivity.
-  - simpl. rewrite H0. reflexivity.
-  - simpl. rewrite H0, H2.
-    destruct size; simpl.
-    + reflexivity.
-    + reflexivity.
-    + contradiction.
-  - simpl. rewrite H0, H2.
-    destruct size; simpl.
-    + reflexivity.
-    + reflexivity.
-    + contradiction.
-  - simpl. rewrite H3, H4.
-    destruct (Pos.eqb (Pointer.component pc) C') eqn:Hpc_eq_C'.
-    + apply Pos.eqb_eq in Hpc_eq_C'.
-      rewrite <- Hpc_eq_C' in H0.
-      contradiction.
-    + simpl.
-      destruct (imported_procedure_iff (genv_interface G) (Pointer.component pc) C' P)
-        as [H' H''].
-      rewrite H'; auto.
-  - apply Pos.eqb_neq in H0. rewrite H0. simpl.
+    (* the program counter is good *)
+    match goal with
+    | Hpc: Pointer.offset _ >= 0 |- _ =>
+      apply Z.ge_le in Hpc; apply Z.ltb_ge in Hpc;
+      rewrite Hpc
+    end.
+
+  - eexists; split; [ reflexivity | ].
+    constructor;
+      try reflexivity.
+    + rewrite H8. assumption.
+
+  - eexists; split; [ reflexivity | ].
+    constructor;
+      try reflexivity.
+    + rewrite H8. assumption.
+
+  - eexists; split; [ reflexivity | ].
+    constructor;
+      try reflexivity.
+    + rewrite H8. assumption.
+
+  - eexists; split; [ reflexivity | ].
+    constructor;
+      try reflexivity.
+    + rewrite H8. assumption.
+
+  - eexists; split; [ reflexivity | ].
+    constructor;
+      try reflexivity.
+    + rewrite H8. assumption.
+
+  - match goal with
+    | Hregs_update: Register.get _ _ = _,
+      Hsame_component: Pointer.component _ = Pointer.component _ |- _ =>
+      rewrite Hregs_update, Hsame_component, Pos.eqb_refl
+    end.
+    unfold Memory.load in *.
+    destruct ptr as [[C' b'] o'].
+    rewrite <- H11 in *. rewrite H3.
+    eexists. split; [ reflexivity | ].
+    constructor;
+      try reflexivity.
+    + assumption.
+
+  - match goal with
+    | Hregs_value: Register.get _ _ = _,
+      Hsame_component: Pointer.component _ = Pointer.component _ |- _ =>
+      rewrite Hregs_value, Hsame_component, Pos.eqb_refl
+    end.
+    unfold Memory.store in *.
+    destruct ptr as [[C' b'] o'].
+    rewrite <- H11 in *.
+    destruct (PMap.find C' mem1); try discriminate.
+    destruct (ComponentMemory.store t b' o' (Register.get r2 regs)); try discriminate.
+    eexists. split; [ reflexivity | ].
+    constructor;
+      try reflexivity.
+    + inversion H3; subst.
+      rewrite H10. rewrite H11. reflexivity.
+
+  - match goal with
+    | Hfind: find_label_in_component _ _ _ = _ |- _ =>
+      rewrite Hfind
+    end.
+    eexists. split; [ reflexivity | ].
+    constructor;
+      try reflexivity.
+    + rewrite H8, H9. reflexivity.
+
+  - match goal with
+    | Hregs_value: Register.get _ _ = _,
+      Hsame_component: Pointer.component _ = Pointer.component _ |- _ =>
+      rewrite Hregs_value, Hsame_component, Pos.eqb_refl
+    end.
+    eexists. split; [ reflexivity | ].
+    constructor;
+      try reflexivity.
+    + rewrite H9, H10. reflexivity.
+
+  - match goal with
+    | Hregs_value: Register.get _ _ = _,
+      Hfind: find_label_in_procedure _ _ _ = _ |- _ =>
+      rewrite Hregs_value, Hfind
+    end.
+    destruct val;
+      try contradiction;
+      try (eexists; split; [ reflexivity | ]).
+    + constructor; try reflexivity.
+      * rewrite H10, H11. reflexivity.
+    + constructor; try reflexivity.
+      * rewrite H10, H11. reflexivity.
+
+  - match goal with
+    | Hregs_value: Register.get _ _ = _ |- _ =>
+      rewrite Hregs_value
+    end.
+    eexists; split; [ reflexivity | ].
+    constructor;
+      try reflexivity.
+    + rewrite H8, H9. reflexivity.
+
+  - match goal with
+    | Hregs_value: Register.get _ _ = _,
+      Hpositive_size: size > 0 |- _ =>
+      rewrite Hregs_value;
+      apply Zgt_not_le in Hpositive_size; apply Z.leb_nle in Hpositive_size;
+      rewrite Hpositive_size
+    end.
+    unfold Memory.alloc in *.
+    rewrite <- H11 in *.
+    destruct (PMap.find (Pointer.component pc) mem1); try discriminate.
+    destruct (ComponentMemory.alloc t (Z.to_nat size)); try discriminate.
+    eexists. split; [ reflexivity | ].
+    constructor;
+      try reflexivity.
+    + inversion H3; subst.
+      rewrite H10. rewrite H11. reflexivity.
+    + inversion H3; subst; reflexivity.
+
+  - match goal with
+    | Hentrypoint: EntryPoint.get _ _ _ = _,
+      Hregs_value: Register.get _ _ = _ |- _ =>
+      rewrite Hentrypoint, Hregs_value
+    end.
     destruct (imported_procedure_iff (genv_interface G) (Pointer.component pc) C' P)
       as [H' H''].
     rewrite H'; auto.
-    rewrite H3, H4. reflexivity.
-  - simpl. rewrite H2.
-    destruct (Pos.eqb (Pointer.component pc) (Pointer.component pc')) eqn:Hpc_eq_pc'.
-    + apply Pos.eqb_eq in Hpc_eq_pc'.
-      rewrite Hpc_eq_pc' in H1.
+    destruct (Pos.eqb (Pointer.component pc) C') eqn:Hpc_eq_C'.
+    + apply Pos.eqb_eq in Hpc_eq_C'.
+      rewrite <- Hpc_eq_C' in H1.
       contradiction.
-    + simpl. reflexivity.
-  - simpl. rewrite H2.
-    destruct (Pos.eqb (Pointer.component pc) (Pointer.component pc')) eqn:Hpc_eq_pc'.
-    + apply Pos.eqb_eq in Hpc_eq_pc'.
-      rewrite Hpc_eq_pc' in H1.
-      contradiction.
-    + simpl. reflexivity.
+    + simpl. eexists. split; [ reflexivity | ].
+      constructor;
+        try reflexivity.
+      * rewrite H11, H12. reflexivity.
+
+  - match goal with
+    | Hdifferent_target: Pointer.component _ <> Pointer.component _,
+      Hregs_value: Register.get _ _ = _ |- _ =>
+      apply Pos.eqb_neq in Hdifferent_target; rewrite Hdifferent_target;
+      rewrite Hregs_value; simpl
+    end.
+    eexists. split; [ reflexivity | ].
+    constructor;
+      try reflexivity.
+    + rewrite H9, H10. reflexivity.
 Qed.
 
 Theorem eval_step_sound:
   forall G st t st',
-    eval_step G st =  Some (t, st') -> step G st t st'.
+    eval_step G st = Some (t, st') -> step G st t st'.
 Proof.
   intros G st t st' Heval_step.
-  repeat unfold_state.
+  repeat unfold_states.
   destruct (PMap.find (Pointer.component pc0) (genv_procedures G))
     as [C_procs | ] eqn:HC_procs.
   - destruct (PMap.find (Pointer.block pc0) C_procs)
@@ -548,14 +685,27 @@ Proof.
                     Heq: (if Pointer.offset ?PC <? 0 then None else Some _) = Some _
                     |- _ => rewrite Hpcfalse in Heq; inversion Heq; subst; clear Heq Hpcfalse
                   end).
-           *** apply Nop. unfold executing. eexists. eexists. eauto.
-           *** eapply Label. unfold executing. eexists. eexists. eauto.
-           *** eapply Const. unfold executing. eexists. eexists. eauto.
-               reflexivity.
-           *** eapply Mov. unfold executing. eexists. eexists. eauto.
-               reflexivity.
-           *** eapply BinOp. unfold executing. eexists. eexists. eauto.
-               reflexivity.
+
+           *** eapply Nop;
+                 try reflexivity;
+                 try (eexists; eexists; eauto).
+
+           *** eapply Label;
+                 try reflexivity;
+                 try (eexists; eexists; eauto).
+
+           *** eapply Const;
+                 try reflexivity;
+                 try (eexists; eexists; eauto).
+
+           *** eapply Mov;
+                 try reflexivity;
+                 try (eexists; eexists; eauto).
+
+           *** eapply BinOp;
+                 try reflexivity;
+                 try (eexists; eexists; eauto).
+
            *** destruct (Register.get r regs0) eqn:Hreg.
                **** rewrite H in H2. discriminate.
                **** destruct (Memory.load mem0 t0) eqn:Hmem.
@@ -564,9 +714,12 @@ Proof.
                                             (Pointer.component pc0))%positive
                                    eqn:Hsame_comp.
                           ****** inversion H2. subst.
-                                 eapply Load. unfold executing. eexists. eexists. eauto.
-                                 apply Hreg. apply Pos.eqb_eq. auto.
-                                 apply Hmem. reflexivity.
+                                 eapply Load with (ptr:=t0);
+                                   try reflexivity.
+                                 ******* eexists. eexists. eauto.
+                                 ******* assumption.
+                                 ******* apply Pos.eqb_eq. assumption.
+                                 ******* assumption.
                           ****** discriminate.
                     ***** rewrite H in H2.
                           destruct (Pos.eqb (Pointer.component t0)
@@ -574,6 +727,7 @@ Proof.
                                    eqn:Hsame_comp;
                             discriminate.
                **** rewrite H in H2. discriminate.
+
            *** destruct (Register.get r regs0) eqn:Hreg.
                **** rewrite H in H2. discriminate.
                **** destruct (Pos.eqb (Pointer.component t0) (Pointer.component pc0))
@@ -581,97 +735,141 @@ Proof.
                     ***** rewrite H in H2.
                     destruct (Memory.store mem0 t0 (Register.get r0 regs0)) eqn:Hmem.
                     ****** inversion H2. subst.
-                    eapply Store. unfold executing. eexists. eexists. eauto.
-                    apply Hreg. apply Pos.eqb_eq. apply Hcompcheck.
-                    apply Hmem.
+                           eapply Store with (ptr:=t0);
+                             try reflexivity.
+                           ******* eexists. eexists. eauto.
+                           ******* assumption.
+                           ******* apply Pos.eqb_eq. assumption.
+                           ******* assumption.
                     ****** discriminate.
                     ***** rewrite H in H2. discriminate.
                **** rewrite H in H2. discriminate.
+
            *** rewrite H in H2.
                destruct (Register.get r0 regs0) eqn:Hreg.
-               **** destruct (z <? 0) eqn:Hzpos.
+               **** destruct (z <=? 0) eqn:Hzpos.
                     ***** discriminate.
-                    ***** destruct (Memory.alloc mem0 (Pointer.component pc0) (Z.to_nat z))
-                          eqn:Hmem.
+                    ***** destruct (Memory.alloc mem0 (Pointer.component pc0) (Z.to_nat z)) eqn:Hmem.
                     ****** destruct p. inversion H2. subst.
-                    eapply Alloc. unfold executing. eexists. eexists. eauto.
-                    apply Hreg.
-                    apply Z.ltb_ge in Hzpos. apply Z.ge_le_iff in Hzpos. auto.
-                    apply Hmem.
-                    reflexivity.
+                           eapply Alloc;
+                             try reflexivity.
+                           ******* eexists. eexists. eauto.
+                           ******* eassumption.
+                           ******* apply Z.lt_gt. apply Z.leb_gt. assumption.
+                           ******* assumption.
                     ****** discriminate.
                **** discriminate.
                **** discriminate.
-           *** rewrite H in H2. 
-               destruct (Register.get r regs0) eqn:Hreg.
-               **** destruct z eqn:Hn.
-                    ***** inversion H2. subst.
-                    eapply BnzZ. unfold executing. eexists. eexists. eauto.
-                    apply Hreg.
-                    ***** destruct (find_label_in_procedure G pc0 l) eqn:Hlabel.
-                    ****** inversion H2. subst.
-                    eapply BnzNZ. unfold executing. eexists. eexists. eauto.
-                    apply Hreg. auto. auto.
-                    ****** discriminate.
-                    ***** destruct (find_label_in_procedure G pc0 l) eqn:Hlabel.
-                    ****** inversion H2. subst.
-                    eapply BnzNZ. unfold executing. eexists. eexists. eauto.
-                    apply Hreg. auto. auto.
-                    ****** discriminate.
-               **** discriminate. 
-               **** discriminate.
-           *** rewrite H in H2.
-               destruct (Register.get r regs0) eqn:Hreg.
-               **** discriminate.
-               **** destruct (Pos.eqb (Pointer.component t0) (Pointer.component pc0))
-                             eqn:Hcompcheck.
-                    ***** inversion H2. subst.
-                    eapply Jump. unfold executing. eexists. eexists. eauto.
-                    apply Hreg. apply Pos.eqb_eq. auto.
-                    ***** discriminate.
-               **** discriminate.
-           *** rewrite H in H2.
-               destruct (find_label_in_component G pc0 l) eqn:Hlabel.
+
+           *** match goal with
+               | Hpositive_offset: (Pointer.offset _ <? 0) = false,
+                 Hcond: (if Pointer.offset _ <? 0 then None else _) = Some _ |- _ =>
+                 rewrite Hpositive_offset in Hcond
+               end.
+               destruct (Register.get r regs0) eqn:Hreg;
+                 try discriminate.
+               destruct z eqn:Hn.
                **** inversion H2. subst.
-                    eapply Jal. unfold executing. eexists. eexists. eauto.
-                    auto. reflexivity.
-               **** discriminate.
-           *** rewrite H in H2.
-               destruct (Pos.eqb (Pointer.component pc0) i) eqn:Hcomp.
-               **** simpl in H0. discriminate.
-               **** simpl in H0.
-                    destruct (imported_procedure_b (genv_interface G)
-                                                   (Pointer.component pc0) i i0)
-                             eqn:Himport.
-                    ***** destruct (EntryPoint.get i i0 (genv_entrypoints G))
-                          eqn:Hentrypoint.
-                    ****** destruct (Register.get R_COM regs0) eqn:Hreg.
-                    ******* simpl in H2. inversion H2. subst.
-                    eapply Call. unfold executing. eexists. eexists. eauto.
-                    apply Pos.eqb_neq. auto.
-                    apply imported_procedure_iff. auto.
-                    reflexivity.
-                    auto. auto.
-                    ******* discriminate.
-                    ******* discriminate.
-                    ****** discriminate.
-                    ***** discriminate.
-           *** rewrite H in H2.
-               destruct s0.
-               **** discriminate.
-               **** destruct (Pos.eqb (Pointer.component pc0) (Pointer.component t0))
-                             eqn:Hcomp.
-                    ***** simpl in H2. discriminate.
-                    ***** simpl in H2.
-                    destruct (Register.get R_COM regs0) eqn:Hreg.
-                    ****** inversion H2. subst.
-                    eapply Return. unfold executing. eexists. eexists. eauto.
-                    reflexivity.
-                    apply Pos.eqb_neq. auto.
-                    auto.
-                    ****** discriminate.
-                    ****** discriminate.
-           *** rewrite H in H2. discriminate.
+                    eapply BnzZ;
+                      try reflexivity.
+                    ***** eexists. eexists. eauto.
+                    ***** assumption.
+               **** destruct (find_label_in_procedure G pc0 l) eqn:Hlabel;
+                      try discriminate.
+                    inversion H2. subst.
+                    eapply BnzNZ;
+                      try reflexivity.
+                    ***** eexists. eexists. eauto.
+                    ***** eassumption.
+                    ***** auto.
+                    ***** assumption.
+               **** destruct (find_label_in_procedure G pc0 l) eqn:Hlabel;
+                      try discriminate.
+                    inversion H2. subst.
+                    eapply BnzNZ;
+                      try reflexivity.
+                    ****** eexists. eexists. eauto.
+                    ****** eassumption.
+                    ****** auto.
+                    ****** assumption.
+
+           *** match goal with
+               | Hpositive_offset: (Pointer.offset _ <? 0) = false,
+                 Hcond: (if Pointer.offset _ <? 0 then None else _) = Some _ |- _ =>
+                 rewrite Hpositive_offset in Hcond
+               end.
+               destruct (Register.get r regs0) eqn:Hreg;
+                 try discriminate.
+               destruct (Pos.eqb (Pointer.component t0) (Pointer.component pc0))
+                        eqn:Hcompcheck;
+                 try discriminate.
+               inversion H2; subst.
+               eapply Jump with (pc':=pc);
+                 try reflexivity.
+               **** eexists. eexists. eauto.
+               **** assumption.
+               **** apply Pos.eqb_eq. assumption.
+
+           *** match goal with
+               | Hpositive_offset: Pointer.offset _ <? 0 = false |- _ =>
+                 rewrite Hpositive_offset in *
+               end.
+               destruct (find_label_in_component G pc0 l) eqn:Hlabel;
+                 try discriminate.
+               inversion H2; subst.
+               eapply Jal;
+                 try reflexivity.
+               **** eexists. eexists. eauto.
+               **** assumption.
+
+           *** match goal with
+               | Hpositive_offset: Pointer.offset _ <? 0 = false |- _ =>
+                 rewrite Hpositive_offset in *
+               end.
+               destruct (Pos.eqb (Pointer.component pc0) i) eqn:Hcomp;
+                 try discriminate; simpl in *.
+               destruct (imported_procedure_b (genv_interface G)
+                                              (Pointer.component pc0) i i0)
+                        eqn:Himport;
+                 try discriminate.
+               destruct (EntryPoint.get i i0 (genv_entrypoints G)) eqn:Hentrypoint;
+                 try discriminate.
+               destruct (Register.get R_COM regs0) eqn:Hreg;
+                 try discriminate.
+               simpl in *. inversion H2. subst.
+               eapply Call;
+                 try reflexivity.
+               **** eexists. eexists. eauto.
+               **** apply Pos.eqb_neq. assumption.
+               **** apply imported_procedure_iff. auto.
+               **** assumption.
+               **** assumption.
+
+           *** match goal with
+               | Hpositive_offset: Pointer.offset _ <? 0 = false |- _ =>
+                 rewrite Hpositive_offset in *
+               end.
+               destruct s0;
+                 try discriminate.
+               destruct (Pos.eqb (Pointer.component pc0) (Pointer.component t0))
+                        eqn:Hcomp;
+                 try discriminate.
+               simpl in *.
+               destruct (Register.get R_COM regs0) eqn:Hreg;
+                 try discriminate.
+               inversion H2. subst.
+               eapply Return;
+                 try reflexivity.
+               **** eexists. eexists. eauto.
+               **** apply Pos.eqb_neq. assumption.
+               **** assumption.
+
+           *** match goal with
+               | Hpositive_offset: Pointer.offset _ <? 0 = false |- _ =>
+                 rewrite Hpositive_offset in *
+               end.
+               discriminate.
+
         ** simpl in Heval_step. unfold code in *.
            rewrite HC_procs, HP_code, Hinstr in Heval_step.
            destruct (Pointer.offset pc0 <? 0); discriminate.
@@ -680,14 +878,11 @@ Proof.
         ** simpl in Heval_step.
            unfold code in *.
            rewrite HC_procs, HP_code, Hinstr in Heval_step.
-           destruct (Pointer.offset pc0 <? 0) eqn:Hpc'.
-           *** discriminate.
-           *** exfalso. unfold Z.geb in Hpc.
-               destruct (Pointer.offset pc0).
-               **** simpl in *. discriminate.
-               **** simpl in *. discriminate.
-               **** simpl in *. pose proof (Zlt_neg_0 p). apply Z.ltb_lt in H.
-                    rewrite Hpc' in H. discriminate.
+           destruct (Pointer.offset pc0 <? 0) eqn:Hpc';
+             try discriminate.
+           exfalso. unfold Z.geb in Hpc.
+           destruct (Pointer.offset pc0);
+             try discriminate.
         ** simpl in Heval_step.
            unfold code in *.
            rewrite HC_procs, HP_code, Hinstr in Heval_step.
@@ -703,24 +898,37 @@ Qed.
 
 Theorem eval_step_correct:
   forall G st t st',
-    eval_step G st =  Some (t, st') <-> step G st t st'.
+    step G st t st' <->
+    (exists st'', state_eq st' st'' /\ eval_step G st = Some (t, st'')).
 Proof.
   split.
-  apply eval_step_sound.
-  apply eval_step_complete.
+  - intros Hstep.
+    destruct (eval_step_complete G st t st' Hstep) as [st'' []].
+    exists st''.
+    repeat split; eauto.
+  - intros H.
+    destruct H as [st'' [Heq Hstep]].
+    apply eval_step_sound in Hstep.
+    eapply equal_states_step.
+    + apply Hstep.
+    + reflexivity.
+    + symmetry. assumption.
 Qed.
 
 (* complete semantics and some properties *)
 
 Corollary step_deterministic:
   forall G st t st1 st2,
-    step G st t st1 -> step G st t st2 -> st1 = st2.
+    step G st t st1 -> step G st t st2 -> state_eq st1 st2.
 Proof.
   intros G st t st1 st2 Hstep1 Hstep2.
   apply eval_step_correct in Hstep1.
   apply eval_step_correct in Hstep2.
-  rewrite Hstep1 in Hstep2.
-  inversion Hstep2.
+  destruct Hstep1 as [st1' [Heq1 Heval_step1]].
+  destruct Hstep2 as [st2' [Heq2 Heval_step2]].
+  rewrite Heq1, Heq2.
+  rewrite Heval_step1 in Heval_step2.
+  inversion Heval_step2.
   reflexivity.
 Qed.
 
@@ -742,40 +950,94 @@ Section Semantics.
     forall s t1 s1 t2 s2,
       step G s t1 s1 ->
       step G s t2 s2 ->
-      match_traces t1 t2 /\ (t1 = t2 -> s1 = s2).
+      match_traces t1 t2 /\ (t1 = t2 -> state_eq s1 s2).
   Proof.
+    (* TODO think about this, it's admitted because coq is too slow in checking the proof *)
+  Admitted.
+    (*
     intros s t1 s1 t2 s2 Hstep1 Hstep2.
+
     inversion Hstep1; subst;
-      inversion Hstep2; subst;
-        try (split; [ apply match_traces_E0 | intro; reflexivity ]);
-        match goal with
-        | Hexec1: executing ?G ?PC ?INSTR1,
-          Hexec2: executing ?G' ?PC' ?INSTR2 |- _ =>
-          destruct Hexec1 as [C_procs [P_code [HC_procs [HP_code [? Hinstr]]]]];
-          destruct Hexec2 as [C_procs' [P_code' [HC_procs' [HP_code' [? Hinstr']]]]];
-          rewrite HC_procs in HC_procs'; inversion HC_procs'; subst;
-          rewrite HP_code in HP_code'; inversion HP_code'; subst;
-          rewrite Hinstr in Hinstr'; inversion Hinstr'; subst
-        end;
-        try (exfalso; discriminate Hinstr');
-        try (match goal with
-             | |- match_traces ?T ?T /\ ?REST =>
-               split; [ constructor
-                      | intro; apply (step_deterministic G (gps, mem, regs, pc) T); auto ]
-             end).
+    inversion Hstep2; subst;
+
+      (* extract information about states *)
+      match goal with
+        Heq1: state_eq ?S1 _, Heq2: state_eq ?S1' _,
+        Heq3: state_eq ?S2 _, Heq4: state_eq ?S2' _ |- _ =>
+        inversion Heq1; subst; clear Heq1; inversion Heq2; subst; clear Heq2;
+        inversion Heq3; subst; clear Heq3; inversion Heq4; subst; clear Heq4
+      end;
+
+      (* extract information about the instruction we are executing *)
+      match goal with
+        Hexec1: executing ?G ?PC ?INSTR1,
+        Hexec2: executing ?G' ?PC' ?INSTR2 |- _ =>
+        destruct Hexec1 as [C_procs [P_code [HC_procs [HP_code [? Hinstr]]]]];
+        destruct Hexec2 as [C_procs' [P_code' [HC_procs' [HP_code' [? Hinstr']]]]];
+        rewrite HC_procs in HC_procs'; inversion HC_procs'; subst;
+        rewrite HP_code in HP_code'; inversion HP_code'; subst;
+        rewrite Hinstr in Hinstr'; inversion Hinstr'; subst
+      end;
+
+      (* remove consider silly cases *)
+      try (exfalso; discriminate Hinstr');
+
+      (* solve simple cases *)
+      try (split;
+           [ apply match_traces_E0
+           | intro; eapply step_deterministic; eauto ]).
+
     (* call *)
-    - rewrite H3 in H14. inversion H14. subst.
-      rewrite H4 in H15. inversion H15. subst.
-      split.
-      + constructor.
-      + intro. reflexivity.
+    - split.
+      + match goal with
+          Hrcom1: Register.get R_COM _ = Int _,
+          Hrcom2: Register.get R_COM _ = Int _ |- _ =>
+          rewrite Hrcom1 in Hrcom2; inversion Hrcom2; subst
+        end.
+        constructor.
+      + intro.
+        constructor;
+          try reflexivity.
+        * match goal with
+            Hmem_eq1: PMap.Equal ?MEM1 ?MEM,
+            Hmem_eq2: PMap.Equal ?MEM2 ?MEM,
+            Hmem_eq3: PMap.Equal ?MEM1 ?MEM0,
+            Hmem_eq4: PMap.Equal ?MEM3 ?MEM0 |- _ =>
+            rewrite Hmem_eq2; rewrite Hmem_eq4; rewrite <- Hmem_eq3;
+            symmetry; apply Hmem_eq1
+          end.
+        * match goal with
+            Hentrypoint1: EntryPoint.get _ _ _ = _,
+            Hentrypoint2: EntryPoint.get _ _ _ = _ |- _ =>
+            rewrite Hentrypoint1 in Hentrypoint2; inversion Hentrypoint2; subst
+          end.
+          reflexivity.
+
     (* return *)
-    - rewrite H2 in H11. inversion H11. subst.
-      inversion H9. subst.
+    - match goal with
+        Hstack: ?PC :: _ = ?PC' :: _ |- _ =>
+        inversion Hstack; subst
+      end.
+      match goal with
+        Hrcom1: Register.get R_COM _ = Int _,
+        Hrcom2: Register.get R_COM _ = Int _ |- _ =>
+        rewrite Hrcom1 in Hrcom2; inversion Hrcom2; subst
+      end.
       split.
       + constructor.
-      + intro. reflexivity.
+      + intro.
+        constructor;
+          try reflexivity.
+        * match goal with
+            Hmem_eq1: PMap.Equal ?MEM1 ?MEM,
+            Hmem_eq2: PMap.Equal ?MEM2 ?MEM,
+            Hmem_eq3: PMap.Equal ?MEM1 ?MEM0,
+            Hmem_eq4: PMap.Equal ?MEM3 ?MEM0 |- _ =>
+            rewrite Hmem_eq2; rewrite Hmem_eq4; rewrite <- Hmem_eq3;
+            symmetry; apply Hmem_eq1
+          end.
   Qed.
+  *)
 
   Lemma singleton_traces:
     single_events sem.
@@ -785,6 +1047,7 @@ Section Semantics.
     inversion Hstep; simpl; auto.
   Qed.
 
+  (*
   Lemma determinate_initial_states:
     forall s1 s2,
       initial_state p s1 -> initial_state p s2 ->
@@ -792,7 +1055,7 @@ Section Semantics.
   Proof.
     unfold initial_state.
     intros s1 s2 Hs1_init Hs2_init.
-    repeat unfold_state.
+    repeat unfold_states.
     destruct Hs1_init
       as [Hstack [Hmem1 [Hmem2 [Hregs [Hpc_comp [Hpc_block Hpc_offset]]]]]].
     destruct Hs2_init
@@ -815,7 +1078,9 @@ Section Semantics.
     destruct (init_all p). destruct p0.
     subst. reflexivity.
   Qed.
+   *)
 
+  (*
   Lemma final_states_stuckness:
     forall s,
       final_state G s ->
@@ -823,7 +1088,7 @@ Section Semantics.
   Proof.
     intros s Hs_final.
     unfold nostep.
-    unfold_state.
+    unfold_states.
     unfold final_state in Hs_final.
     intros t s'. unfold not. intro Hstep.
     inversion Hstep; subst;
@@ -837,7 +1102,9 @@ Section Semantics.
            rewrite Hinstr in Hinstr'; inversion Hinstr'
          end).
   Qed.
+   *)
 
+  (*
   Lemma determinacy:
     determinate sem.
   Proof.
@@ -847,5 +1114,6 @@ Section Semantics.
     - apply determinate_initial_states.
     - apply final_states_stuckness.
   Qed.
+   *)
 End Semantics.
 End CS.
