Intermediate/Composition.v
@@ -11,7 +11,6 @@ Require Import Intermediate.CS.
 Require Import Intermediate.PS.
 Require Import Intermediate.Decomposition.
 
-Import GlobalEnv.
 Import Intermediate.
 
 Section PS2CS.
@@ -79,22 +78,17 @@ Section PS2CS.
       try contradiction.
     inversion H11; subst.
 
-    assert (CS.state_eq (gps0, mem0, regs, pc) (gps, mem, regs, pc)). {
-      constructor; try reflexivity.
-      - rewrite (PS.to_partial_stack_with_empty_context gps gps0); auto.
-      - rewrite H0 in H10.
+    eapply CS.equal_states_step in H1.
+    - eexists. split. apply H1. apply H3.
+    - constructor; try reflexivity.
+      + rewrite (PS.to_partial_stack_with_empty_context gps gps0); auto.
+      + rewrite H0 in H10.
         unfold PMap.Equal, PMapExtra.filter in *.
         intros C. specialize (H10 C).
         rewrite PMapExtra.fold_identity in H10.
         rewrite PMapExtra.fold_identity in H10.
         auto.
-    }
-
-    destruct (CS.equal_states_step G (gps0, mem0, regs, pc) t ics'
-                                   (gps, mem, regs, pc) H4 H1) as [ics'' [Hstep' Heq']].
-    eexists ics''.
-    split; auto.
-    eapply PS.equal_states_partialize; eauto.
+    - reflexivity.
   Qed.
 
   Lemma star_simulation:
@@ -144,7 +138,7 @@ Section PS2CS.
     intros.
 
     (* manually prove that PS is going wrong *)
-    
+
     destruct (forward_simulation_behavior_improves CS_simulates_PS H)
       as [beh' [Hbeh []]]; subst; auto.
 
@@ -167,7 +161,7 @@ Section PS2CS.
         * unfold not. intros.
           apply H8. econstructor; eauto.
           ** PS.simplify_turn. unfold not. intro.
-             destruct s'. repeat destruct p. 
+             destruct s'. repeat destruct p.
              eapply PMapFacts.empty_in_iff in H11; inversion H11.
              destruct c. destruct p.
              eapply PMapFacts.empty_in_iff in H11; inversion H11.
@@ -182,6 +176,518 @@ Section PS2CS.
   Qed.
 End PS2CS.
 
+(*** experimental ***)
+
+(*
+   IDEA:
+   - the context simulates the program, we change our point view on the simulation
+     whenever the control changes
+   - a star in the partial semantics is splitted into a mt_star, that is,
+     a sequence of st_star (a star in which the turn remains the same) connected by
+     single steps that change control
+*)
+
+Inductive same_turn: PS.state -> PS.state -> Prop :=
+| same_turn_program: forall prog_st prog_st',
+    same_turn (PS.PC prog_st) (PS.PC prog_st')
+| same_turn_context: forall ctx_st ctx_st',
+    same_turn (PS.CC ctx_st) (PS.CC ctx_st').
+
+(* st_star represents a sequence of events performed by the same actor *)
+(* st stands for same turn *)
+Inductive st_star (G: global_env) (ctx: Program.interface)
+  : PS.state -> trace -> PS.state -> Prop :=
+| st_star_refl: forall ips,
+    st_star G ctx ips E0 ips
+| st_star_step: forall ips t1 ips' t2 ips'' t,
+    PS.step ctx G ips t1 ips' ->
+    same_turn ips ips' ->
+    st_star G ctx ips' t2 ips'' ->
+    same_turn ips' ips'' ->
+    t = t1 ** t2 ->
+    st_star G ctx ips t ips''.
+
+Lemma st_star_same_turn:
+  forall G ctx ips t ips',
+    st_star G ctx ips t ips' ->
+    same_turn ips ips'.
+Proof.
+  intros G ctx ips t ips' Hst_star.
+  induction Hst_star; subst.
+  - PS.unfold_states; constructor.
+  - repeat PS.unfold_states;
+      try constructor;
+      match goal with
+      | contra: same_turn (PS.CC _) (PS.PC _) |- _ =>
+        inversion contra
+      | contra: same_turn (PS.PC _) (PS.CC _) |- _ =>
+        inversion contra
+      end.
+Qed.
+
+(* mt_star is a sequence of st_star interleaved by steps that change control *)
+(* mt stands for multi turn *)
+Inductive mt_star (G: global_env) (ctx: Program.interface)
+  : PS.state -> trace -> PS.state -> Prop :=
+| mt_star_segment: forall ips t ips',
+    st_star G ctx ips t ips' ->
+    mt_star G ctx ips t ips'
+| mt_star_control_change: forall ips t1 ips' t2 ips'' t3 ips''' t,
+    st_star G ctx ips t1 ips' ->
+    PS.step ctx G ips' t2 ips'' ->
+    ~ same_turn ips' ips'' ->
+    mt_star G ctx ips'' t3 ips''' ->
+    t = t1 ** t2 ** t3 ->
+    mt_star G ctx ips t ips'''.
+
+Theorem star_if_st_star:
+  forall G ctx ips t ips',
+    st_star G ctx ips t ips' ->
+    star (PS.step ctx) G ips t ips'.
+Proof.
+  intros G ctx ips t ips' Hst_star.
+  induction Hst_star; subst.
+  - constructor.
+  - econstructor.
+    + eassumption.
+    + eassumption.
+    + reflexivity.
+Qed.
+
+Theorem star_if_mt_star:
+  forall G ctx ips t ips',
+    mt_star G ctx ips t ips' ->
+    star (PS.step ctx) G ips t ips'.
+Proof.
+  intros G ctx ips t ips' Hmt_star.
+  induction Hmt_star; subst.
+
+  (* st_star *)
+  - apply star_if_st_star; auto.
+
+  (* st_star + step that changes control + mt_star *)
+  - eapply star_trans.
+    + eapply star_right.
+      * apply star_if_st_star. eassumption.
+      * eassumption.
+      * reflexivity.
+    + eassumption.
+    + apply app_assoc.
+Qed.
+
+(* We want to prove that a star is either a sequence of steps without change of control,
+   or it can be decomposed in a star without change of control + a step with the change of control +
+   another star doing the remaining trace *)
+(* how can we prove this? *)
+(* classically? *)
+Lemma change_of_turn_in_star:
+  forall G ctx ips t ips',
+    star (PS.step ctx) G ips t ips' ->
+  st_star G ctx ips t ips' \/
+  (exists ips'' ips''' t1 t2 t3,
+     st_star G ctx ips t1 ips'' /\
+     PS.step ctx G ips'' t2 ips''' /\
+     ~ same_turn ips'' ips''' /\
+     star (PS.step ctx) G ips''' t3 ips' /\
+     t = t1 ** t2 ** t3).
+Proof.
+Admitted.
+
+Theorem mt_star_if_star:
+  forall G ctx ips t ips',
+    star (PS.step ctx) G ips t ips' ->
+    mt_star G ctx ips t ips'.
+Proof.
+  intros G ctx ips t ips' Hstar.
+
+  induction Hstar; subst.
+
+  (* base case, no steps *)
+  - apply mt_star_segment.
+    apply st_star_refl.
+
+  (* step + star *)
+  - PS.unfold_state s1; PS.unfold_state s2.
+
+    (* PC to PC *)
+    + destruct (change_of_turn_in_star G ctx (PS.PC (pgps0, pmem0, regs0, pc0)) t2 s3 Hstar)
+        as [ | [s2' [s2'' [t2' [t2'' [t2'''
+               [Hfirst_st_star [Hstep [Hdiff_turn [Hremaining_star Htrace]]]]]]]]]].
+      * apply mt_star_segment.
+        eapply st_star_step.
+        ** eassumption.
+        ** constructor.
+        ** eassumption.
+        ** eapply st_star_same_turn; eassumption.
+        ** reflexivity.
+      * eapply mt_star_control_change.
+        ** eapply st_star_step.
+           *** eassumption.
+           *** constructor.
+           *** apply Hfirst_st_star.
+           *** eapply st_star_same_turn; eassumption.
+           *** reflexivity.
+        ** apply Hstep.
+        ** assumption.
+        ** admit.
+        ** admit.
+
+    (* PC to CC *)
+    + eapply mt_star_control_change.
+      * apply st_star_refl.
+      * eassumption.
+      * intro contra. inversion contra.
+      * eassumption.
+      * reflexivity.
+
+    (* CC to PC *)
+    + eapply mt_star_control_change.
+      * apply st_star_refl.
+      * eassumption.
+      * intro contra. inversion contra.
+      * eassumption.
+      * reflexivity.
+
+    (* CC to CC *)
+    + admit.
+Admitted.
+
+Theorem star_mt_star_equivalence:
+  forall G ctx ips t ips',
+    star (PS.step ctx) G ips t ips' <-> mt_star G ctx ips t ips'.
+Proof.
+  intros.
+  split.
+  - apply mt_star_if_star.
+  - apply star_if_mt_star.
+Qed.
+
+(*** Internal simulation, context simulates program ***)
+
+Module ProgramSem.
+Section Semantics.
+  Variable prog: program.
+  Variable ctx: Program.interface.
+
+  Inductive initial_state : PS.state -> Prop :=
+  | initial_state_intro: forall ips,
+      PS.is_program_component ips ctx ->
+      initial_state ips.
+
+  Inductive final_state : PS.state -> Prop :=
+  | final_state_nostep: forall ips,
+      PS.is_program_component ips ctx ->
+      Nostep (PS.sem prog ctx) ips ->
+      final_state ips
+  | final_state_step_into_context: forall ips t ips',
+      PS.is_program_component ips ctx ->
+      PS.is_context_component ips' ctx ->
+      Step (PS.sem prog ctx) ips t ips' ->
+      final_state ips.
+
+  Definition sem :=
+    @Semantics_gen PS.state global_env (PS.step ctx)
+                   initial_state final_state (init_genv prog).
+End Semantics.
+End ProgramSem.
+
+Module ContextSem.
+Section Semantics.
+  Variable prog: program.
+  Variable ctx: Program.interface.
+
+  Inductive initial_state : PS.state -> Prop :=
+  | initial_state_intro: forall ips,
+      PS.is_context_component ips ctx ->
+      initial_state ips.
+
+  Inductive final_state : PS.state -> Prop :=
+  | final_state_intro: forall ips,
+      PS.is_context_component ips ctx ->
+      final_state ips.
+
+  Definition sem :=
+    @Semantics_gen PS.state global_env (PS.step ctx)
+                   initial_state final_state (init_genv prog).
+End Semantics.
+End ContextSem.
+
+Module ProgCtxSim.
+Section Simulation.
+  Variable prog1 prog2: program.
+
+  Hypothesis same_main:
+    prog_main prog1 = prog_main prog2.
+
+  Hypothesis disjointness:
+    PMapExtra.Disjoint (prog_interface prog1) (prog_interface prog2).
+
+  Lemma match_initial_states:
+    forall ips1,
+      ProgramSem.initial_state (prog_interface prog2) ips1 ->
+    exists ips2,
+      ContextSem.initial_state (prog_interface prog1) ips2 /\
+      PS.mergeable_states (prog_interface prog1) (prog_interface prog2) ips1 ips2.
+  Proof.
+  Admitted.
+
+  Lemma match_final_states:
+    forall ips1 ips2,
+      PS.mergeable_states (prog_interface prog1) (prog_interface prog2) ips1 ips2 ->
+      ProgramSem.final_state prog1 (prog_interface prog2) ips1 ->
+      ContextSem.final_state (prog_interface prog1) ips2.
+  Proof.
+  Admitted.
+
+  Lemma lockstep_simulation:
+    forall ips1 t ips1',
+      Step (ProgramSem.sem prog1 (prog_interface prog2)) ips1 t ips1' ->
+    forall ips2,
+      PS.mergeable_states (prog_interface prog1) (prog_interface prog2) ips1 ips2 ->
+    exists ips2',
+      Step (ContextSem.sem prog2 (prog_interface prog1)) ips2 t ips2' /\
+      PS.mergeable_states (prog_interface prog1) (prog_interface prog2) ips1' ips2'.
+  Proof.
+  Admitted.
+
+  Theorem context_simulates_program:
+    forward_simulation (ProgramSem.sem prog1 (prog_interface prog2))
+                       (ContextSem.sem prog2 (prog_interface prog1)).
+  Proof.
+    eapply forward_simulation_step.
+    - apply match_initial_states.
+    - apply match_final_states.
+    - apply lockstep_simulation.
+  Qed.
+End Simulation.
+End ProgCtxSim.
+
+Module MultiSem.
+Section MultiSemantics.
+  Variable prog1 prog2: program.
+
+  Hypothesis same_main:
+    prog_main prog1 = prog_main prog2.
+
+  Hypothesis disjointness:
+    PMapExtra.Disjoint (prog_interface prog1) (prog_interface prog2).
+
+  Let prog := program_link prog1 prog2 (fst (prog_main prog1)) (snd (prog_main prog1)).
+  Let empty_ctx := PMap.empty Component.interface.
+  Let G := init_genv prog.
+
+  Definition mstate : Type := PS.state * PS.state.
+
+  Inductive minitial_state : mstate -> Prop :=
+  | initial_state_intro: forall ips1 ips2,
+      PS.mergeable_states (prog_interface prog2) (prog_interface prog1) ips1 ips2 ->
+      PS.initial_state prog1 (prog_interface prog2) ips1 ->
+      PS.initial_state prog2 (prog_interface prog1) ips2 ->
+      minitial_state (ips1, ips2).
+
+  Inductive mfinal_state : mstate -> Prop :=
+  | final_state_intro: forall ips1 ips2,
+      PS.final_state prog1 (prog_interface prog2) ips1 ->
+      PS.final_state prog2 (prog_interface prog1) ips2 ->
+      mfinal_state (ips1, ips2).
+
+  Inductive mstep (G: global_env)
+    : mstate -> trace -> mstate -> Prop :=
+  | multi_step: forall ips1 t ips1' ips2 ips2',
+      PS.step (prog_interface prog2) G ips1 t ips1' ->
+      PS.step (prog_interface prog1) G ips2 t ips2' ->
+      mstep G (ips1, ips2) t (ips1', ips2').
+
+  Definition msem :=
+    @Semantics_gen mstate global_env
+                   mstep minitial_state
+                   mfinal_state G.
+
+  Inductive multi_match : mstate -> PS.state -> Prop :=
+  | multi_match_intro: forall ips1 ips2,
+      PS.mergeable_states (prog_interface prog2) (prog_interface prog1) ips1 ips2 ->
+      multi_match (ips1, ips2) (PS.merge_partial_states ips1 ips2).
+
+  Lemma multi_match_initial_states:
+    forall ms,
+      minitial_state ms ->
+    exists ips,
+      PS.initial_state prog empty_ctx ips /\ multi_match ms ips.
+  Proof.
+    intros ms Hms_init.
+    inversion Hms_init; subst.
+    exists (PS.merge_partial_states ips1 ips2).
+    split.
+    - apply PS.initial_state_intro
+        with (ics:=PS.unpartialize (PS.merge_partial_states ips1 ips2)).
+      + inversion H0; subst. inversion H1; subst.
+        inversion H2; subst; inversion H4; subst; PS.simplify_turn.
+        * (* contra *)
+          inversion H.
+        * econstructor.
+          ** PS.simplify_turn.
+             intro contra. eapply PMapFacts.empty_in_iff; eauto.
+          ** simpl. rewrite Memory.filter_identity. reflexivity.
+          ** simpl.
+             rewrite PS.to_partial_stack_unpartialize_identity.
+             *** reflexivity.
+             *** apply PS.merged_stack_has_no_holes.
+                 inversion H; subst. assumption.
+        * econstructor.
+          ** PS.simplify_turn.
+             intro contra. eapply PMapFacts.empty_in_iff; eauto.
+          ** simpl. rewrite Memory.filter_identity. reflexivity.
+          ** simpl.
+             rewrite PS.to_partial_stack_unpartialize_identity.
+             *** reflexivity.
+             *** apply PS.merged_stack_has_no_holes.
+                 inversion H; subst. assumption.
+        * (* contra *)
+          inversion H.
+      + (* unpartilizing the merge preserves the state information that make
+           CS.initial_state true *)
+        inversion H0; subst. inversion H1; subst.
+        inversion H3; subst. inversion H5; subst.
+        inversion H2; subst; inversion H4; subst; PS.simplify_turn.
+        * (* contra *)
+          inversion H.
+        * constructor;
+            try reflexivity.
+          ** (* prove lemma about init_all with larger program *) admit.
+          ** assumption.
+          ** (* prove lemma about EntryPoint.get with larger program *) admit.
+          ** assumption.
+        * constructor;
+            try reflexivity.
+          ** (* prove lemma about init_all with larger program *) admit.
+          ** rewrite H13. simpl.
+             rewrite same_main. reflexivity.
+          ** (* prove lemma about EntryPoint.get with larger program *) admit.
+          ** assumption.
+        * (* contra *)
+          inversion H.
+    - constructor.
+      + assumption.
+  Admitted.
+
+  Lemma multi_match_final_states:
+    forall ms ips,
+      multi_match ms ips ->
+      mfinal_state ms ->
+      PS.final_state prog empty_ctx ips.
+  Proof.
+    intros ms ips Hmmatch Hms_final.
+    inversion Hms_final; subst.
+    inversion Hmmatch; subst.
+    eapply PS.final_state_program
+      with (ics:=PS.unpartialize (PS.merge_partial_states ips1 ips2));
+      inversion H4; subst; PS.simplify_turn.
+    - intro contra. eapply PMapFacts.empty_in_iff; eauto.
+    - intro contra. eapply PMapFacts.empty_in_iff; eauto.
+    - constructor.
+      + PS.simplify_turn.
+        intro contra. eapply PMapFacts.empty_in_iff; eauto.
+      + simpl. rewrite Memory.filter_identity. reflexivity.
+      + simpl.
+        rewrite PS.to_partial_stack_unpartialize_identity.
+        * reflexivity.
+        * apply PS.merged_stack_has_no_holes.
+          inversion H; subst; assumption.
+    - constructor.
+      + PS.simplify_turn.
+        intro contra. eapply PMapFacts.empty_in_iff; eauto.
+      + simpl. rewrite Memory.filter_identity. reflexivity.
+      + simpl.
+        rewrite PS.to_partial_stack_unpartialize_identity.
+        * reflexivity.
+        * apply PS.merged_stack_has_no_holes.
+          inversion H; subst; assumption.
+    - inversion H; subst.
+      + unfold CS.final_state in H8. CS.unfold_states.
+        inversion H7; subst.
+        (* execution in a larger program *)
+        admit.
+      + PS.simplify_turn. contradiction.
+    - inversion H0; subst.
+      + unfold CS.final_state in H8. CS.unfold_states.
+        inversion H7; subst.
+        (* execution in a larger program *)
+        admit.
+      + PS.simplify_turn. contradiction.
+  Admitted.
+
+  Lemma lockstep_simulation:
+    forall ms t ms',
+      mstep G ms t ms' ->
+    forall ips,
+      multi_match ms ips ->
+    exists ips',
+      PS.step empty_ctx G ips t ips' /\ multi_match ms' ips'.
+  Proof.
+    intros ms t ms' Hstep.
+    intros ips Hmatch.
+
+    inversion Hmatch; subst.
+    inversion Hstep; subst.
+
+    exists (PS.merge_partial_states ips1' ips2'). split.
+    - inversion H; subst; simpl.
+      inversion H2; subst. inversion H5; subst.
+      + eapply PS.partial_step with
+            (ics:=PS.unpartialize (PS.PC (PS.merge_stacks pgps1 pgps2,
+                                          PS.merge_memories pmem1 pmem2, regs, pc)))
+            (ics':=PS.unpartialize (PS.merge_partial_states ips1' ips2')).
+        * inversion H8; subst; inversion H11; subst;
+            PS.simplify_turn; simpl in *.
+          ** (* contra, executing component is outside of prog *)
+             admit.
+          ** (* program is in the first state *) admit.
+          ** (* prgroam is in the second state *) admit.
+          ** (* contra, executing component is in both prog1 and prog2 *)
+             exfalso. eapply disjointness. split; eauto.
+             admit.
+        * simpl. constructor; simpl.
+          ** PS.simplify_turn.
+             intro contra.
+             eapply PMapFacts.empty_in_iff; eauto.
+          ** symmetry. apply Memory.filter_identity.
+          ** rewrite PS.to_partial_stack_unpartialize_identity.
+             *** reflexivity.
+             *** apply PS.merged_stack_has_no_holes; auto.
+        * inversion H8; subst; inversion H11; subst;
+            PS.simplify_turn; simpl in *.
+          ** (* contra, executing component is outside of prog *)
+             admit.
+          ** (* program is in the first state *) admit.
+          ** (* prgroam is in the second state *) admit.
+          ** (* contra, executing component is in both prog1 and prog2 *)
+             exfalso. eapply disjointness. split; eauto.
+             admit.
+
+      + (* symmetric the previous case *)
+        admit.
+
+    - inversion H; subst.
+      inversion H2; subst; inversion H5; subst.
+      + inversion H8; subst; inversion H11; subst.
+         ** admit.
+         ** admit.
+         ** admit.
+         ** admit.
+      + admit.
+  Admitted.
+
+  Theorem merged_prog_simulates_multisem:
+    forward_simulation msem (PS.sem prog (PMap.empty Component.interface)).
+  Proof.
+    eapply forward_simulation_step.
+    - apply multi_match_initial_states.
+    - apply multi_match_final_states.
+    - apply lockstep_simulation.
+  Qed.
+End MultiSemantics.
+End MultiSem.
+
 Section PartialComposition.
   Variable prog1 prog2: program.
 
@@ -191,176 +697,203 @@ Section PartialComposition.
   Hypothesis disjointness:
     PMapExtra.Disjoint (prog_interface prog1) (prog_interface prog2).
 
-  (* at some point we will have to use the fact that the link gives us a good program *)
-  (*
-  Hypothesis closedness:
-    closed_program (program_link prog1 prog2 (fst (prog_main prog1)) (snd (prog_main prog1))).
-*)
-
   Let prog := program_link prog1 prog2 (fst (prog_main prog1)) (snd (prog_main prog1)).
   Let empty_ctx := PMap.empty Component.interface.
   Let G := init_genv prog.
 
-  Definition multi_state : Type := PS.state * PS.state.
+  (* with multisem *)
 
-  Inductive multi_initial_state: multi_state -> Prop :=
-  | multi_initial_state_intro: forall ics ips1 ips2,
-      PS.partial_state (prog_interface prog2) ics ips1 ->
-      PS.partial_state (prog_interface prog1) ics ips2 ->
-      PS.mergeable_states ips1 ips2 ->
-      CS.initial_state prog ics ->
-      multi_initial_state (ips1, ips2).
-
-  Inductive multi_final_state : multi_state -> Prop :=
-  | multi_final_state_intro: forall ics ips1 ips2,
-      PS.partial_state (prog_interface prog2) ics ips1 ->
-      PS.partial_state (prog_interface prog1) ics ips2 ->
-      PS.mergeable_states ips1 ips2 ->
-      CS.final_state G ics ->
-      multi_final_state (ips1, ips2).
-
-  Inductive multi_step (G: global_env)
-    : multi_state -> trace -> multi_state -> Prop :=
-  | mstep: forall ips1 t ips1' ips2 ips2',
-      PS.step (prog_interface prog2) G ips1 t ips1' ->
-      PS.step (prog_interface prog1) G ips2 t ips2' ->
-      PS.mergeable_states ips1 ips2 ->
-      multi_step G (ips1, ips2) t (ips1', ips2').
-
-  Definition multisem :=
-    @Semantics_gen multi_state global_env
-                   multi_step multi_initial_state multi_final_state G.
-
-  Inductive multi_match : multi_state -> PS.state -> Prop :=
-  | mmatch_first: forall ips1 ips2,
-      PS.is_program_component ips1 (prog_interface prog2) ->
-      PS.is_context_component ips2 (prog_interface prog1) ->
-      PS.mergeable_states ips1 ips2 ->
-      multi_match (ips1, ips2) (PS.merge_partial_states ips1 ips2)
-  | mmatch_second: forall ips1 ips2,
-      PS.is_context_component ips1 (prog_interface prog2) ->
-      PS.is_program_component ips2 (prog_interface prog1) ->
-      PS.mergeable_states ips1 ips2 ->
-      multi_match (ips1, ips2) (PS.merge_partial_states ips1 ips2).
-
-  (* if ics is a partial state of ips1 and ips2 in, respectively, ctx1 and ctx2,
-     it means that it is also a partial state of the merge of ips1 and ips2 in
-     the empty context *)
-  Lemma merged_state_preserves_partiality:
-    forall ips1 ips2 ics,
-      PS.partial_state (prog_interface prog2) ics ips1 ->
-      PS.partial_state (prog_interface prog1) ics ips2 ->
-      PS.partial_state empty_ctx ics (PS.merge_partial_states ips1 ips2).
+  Lemma threeway_multisem_st_star_simulation:
+    forall ips1 ips2 t ips1' ips2',
+      PS.mergeable_states (prog_interface prog2) (prog_interface prog1) ips1 ips2 ->
+      st_star G (prog_interface prog2) ips1 t ips1' ->
+      st_star G (prog_interface prog1) ips2 t ips2' ->
+      star (MultiSem.mstep prog1 prog2) G (ips1, ips2) t (ips1', ips2') /\
+      PS.mergeable_states (prog_interface prog2) (prog_interface prog1) ips1' ips2'.
   Proof.
+    intros ips1 ips2 t ips1' ips2'.
+    intros Hmergeable Hst_star1 Hst_star2.
+
+    induction Hmergeable; subst.
+
+    (* the programs is in the first state *)
+    (*
+    - remember (PS.PC (pgps1, pmem1, regs, pc)) as ips1.
+      remember (PS.CC (Pointer.component pc, pgps2, pmem2)) as ips2.
+      induction Hst_star1; subst.
+      + apply star_if_st_star in Hst_star2.
+        eapply PS.context_epsilon_star_is_silent in Hst_star2.
+        * split.
+          ** admit.
+          ** admit.
+        * econstructor; try reflexivity.
+
+      + discriminate.
+     *)
+    admit.
+
+    (* the program is in the second state *)
+    (* (should be symmetric w.r.t. the first part of the proof) *)
+    - admit.
   Admitted.
 
-  Lemma partial_state_weakening:
-    forall ips1 ips2 ics,
-      PS.partial_state (prog_interface prog2) ics ips1 ->
-      PS.partial_state empty_ctx ics (PS.merge_partial_states ips1 ips2).
+  Theorem threeway_multisem_mt_star_simulation:
+    forall ips1 ips2 t ips1' ips2',
+      PS.mergeable_states (prog_interface prog2) (prog_interface prog1) ips1 ips2 ->
+      mt_star G (prog_interface prog2) ips1 t ips1' ->
+      mt_star G (prog_interface prog1) ips2 t ips2' ->
+      star (MultiSem.mstep prog1 prog2) G (ips1, ips2) t (ips1', ips2') /\
+      PS.mergeable_states (prog_interface prog2) (prog_interface prog1) ips1' ips2'.
   Proof.
-  Admitted.
+    intros ips1 ips2 t ips1' ips2'.
+    intros Hmergeable Hmt_star1 Hmt_star2.
 
-  (* after the merge, the context will never execute *)
-  Lemma merged_state_always_executes_the_program:
-    forall ips1 ips2,
-      PS.mergeable_states ips1 ips2 ->
-      PS.is_program_component (PS.merge_partial_states ips1 ips2) empty_ctx.
-  Proof.
-  Admitted.
+    induction Hmergeable; subst.
 
-  Lemma multi_match_initial_states:
-    forall ms,
-      multi_initial_state ms ->
-    exists ips,
-      PS.initial_state prog empty_ctx ips /\ multi_match ms ips.
-  Proof.
-    intros ms Hms_init.
-    inversion Hms_init; subst.
-    exists (PS.merge_partial_states ips1 ips2). split.
-    - econstructor; eauto.
-      + eapply merged_state_preserves_partiality; eauto.
-    - (* case analysis how who has control *)
-      CS.unfold_state.
-      destruct (PMap.mem (Pointer.component pc) (prog_interface prog2)) eqn:Hcontrol;
-        [ apply PMapFacts.mem_in_iff in Hcontrol |
-          apply PMapFacts.not_mem_in_iff in Hcontrol ].
-      + apply mmatch_second; auto.
-        * inversion H; subst; inversion H; subst; PS.simplify_turn;
-            try contradiction; auto.
-        * inversion H0; subst; inversion H; subst; PS.simplify_turn; auto.
-          inversion H; subst; inversion H0; subst; PS.simplify_turn; auto.
-          exfalso.
-          apply (disjointness (Pointer.component pc)). split; auto.
-      + apply mmatch_first; auto.
-        * inversion H; subst; inversion H; subst; PS.simplify_turn;
-            try contradiction; auto.
-        * inversion H0; subst; inversion H; subst; PS.simplify_turn; auto.
-          inversion H; subst; inversion H0; subst; PS.simplify_turn; auto.
-          (* Pointer.component pc isn't in ctx1, nor it is in ctx2, that should be
-             impossible *)
-          (* notice that we know Pointer.component pc to be equal to (fst (prog_main p)) *)
-          destruct H2 as [? [? [? [Hpc []]]]].
-          (*
-          destruct closedness as [Hclosed_interface Hmain_existence].
-          destruct Hmain_existence as [mainC_procs []].
-          simpl in *.*)
+    (*
+    (* the programs is in the first state *)
+    - remember (PS.PC (pgps1, pmem1, regs, pc)) as ips.
+      induction Hmt_star1; subst.
+
+      (* single segment *)
+      + inversion Hmt_star2; subst.
+
+        (* single segment with the same trace *)
+        * apply threeway_multisem_st_star_simulation; auto.
+          ** constructor; auto.
+
+        (* segment + change of control (PC to CC) + mt_star *)
+        (* contradiction, the segment is invalid *)
+        * inversion H4.
+
+        (* segment + change of control (CC to PC) + mt_star *)
+        * (* this case is impossible:
+             we have a segment made by the program with trace (t1 ** t2 ** t3) in
+             which there is no change of control.
+             we also a step from context to program with trace t2 that happens after
+             segment made by the context with trace t1.
+             this means that t2 is an event that changes control and we shouldn't be
+             able to observe it inside the program segment. *)
           admit.
+
+      (* segment + change of control (PC to CC) + mt_star *)
+      + inversion Hmt_star2; subst.
+        * (* this case is impossible for the same reason the case above it is impossible.
+             t2 is an event that changes control, it cannot appear inside a segment *)
+          admit.
+        * destruct IHHmt_star1 as [Hstar Hmergeable].
+          ** admit.
+          ** admit.
+          ** admit.
+          ** split.
+             *** eapply star_step.
+                 **** econstructor.
+                      ***** admit.
+                      ***** admit.
+                 **** apply Hstar.
+                 **** admit.
+             *** auto.
+        * (* there are different cases to analyze, there interesting one t0 = t1, t2=t4 *)
+          (* can we prove that it is indeed the only case? *)
+          admit.
+
+      (* segment + change of control (CC to PC) + mt_star *)
+      (* contradiction, the segment is invalid *)
+      + inversion H1.
+
+    (* the program is in the second state *)
+    (* (should be symmetric w.r.t. the first part of the proof) *)
+    - admit.
+     *)
   Admitted.
 
-  Lemma multi_match_final_states:
-    forall ms ips,
-      multi_match ms ips ->
-      multi_final_state ms ->
-      PS.final_state prog empty_ctx ips.
+  Corollary threeway_multisem_star:
+    forall ips1 ips2 t ips1' ips2',
+      PS.mergeable_states (prog_interface prog2) (prog_interface prog1) ips1 ips2 ->
+      star (PS.step (prog_interface prog2)) G ips1 t ips1' ->
+      star (PS.step (prog_interface prog1)) G ips2 t ips2' ->
+      star (MultiSem.mstep prog1 prog2) G (ips1, ips2) t (ips1', ips2').
   Proof.
-    intros ms ips Hmmatch Hms_final.
-    inversion Hms_final; subst.
-    inversion Hmmatch; subst.
-    - eapply PS.final_state_program; eauto.
-      + apply merged_state_always_executes_the_program; auto.
-      + eapply merged_state_preserves_partiality; eauto.
-    - eapply PS.final_state_program; eauto.
-      + apply merged_state_always_executes_the_program; auto.
-      + eapply merged_state_preserves_partiality; eauto.
-  Qed.
-
-  Lemma threeway_simulation:
-    forall ms t ms',
-      multi_step G ms t ms' ->
-    forall ips,
-      multi_match ms ips ->
-    exists ips',
-      PS.step empty_ctx G ips t ips' /\ multi_match ms' ips'.
-  Proof.
-    intros ms t ms' Hstep.
-    intros ips Hmatch.
-
-    inversion Hstep; subst.
-
-    exists (PS.merge_partial_states ips1' ips2'). split.
-    - inversion H; subst.
-      inversion Hmatch; subst;
-        econstructor; eauto; apply partial_state_weakening; auto.
-    - (* case analysis how who has control *)
-  Admitted.
-
-  Theorem prog_simulates_prog1_and_prog2:
-    forward_simulation multisem (PS.sem prog (PMap.empty Component.interface)).
-  Proof.
-    eapply forward_simulation_step.
-    - apply multi_match_initial_states.
-    - apply multi_match_final_states.
-    - apply threeway_simulation.
+    intros ips1 ips2 t ips1' ips2'.
+    intros Hmergeable Hstar1 Hstar2.
+    apply threeway_multisem_mt_star_simulation.
+    - assumption.
+    - apply star_mt_star_equivalence; auto.
+    - apply star_mt_star_equivalence; auto.
   Qed.
 
   Corollary partial_programs_composition:
-    forall beh,
-      program_behaves (PS.sem prog1 (prog_interface prog2)) beh ->
-      program_behaves (PS.sem prog2 (prog_interface prog1)) beh ->
-      program_behaves (PS.sem prog empty_ctx) beh.
+    forall t,
+      program_behaves (PS.sem prog1 (prog_interface prog2)) (Terminates t) ->
+      program_behaves (PS.sem prog2 (prog_interface prog1)) (Terminates t) ->
+      program_behaves (PS.sem prog empty_ctx) (Terminates t).
   Proof.
-    (* this should be provable, but it might be tricky *)
+    intros t Hprog1_beh Hprog2_beh.
+    inversion Hprog1_beh; subst. inversion H0; subst.
+    inversion Hprog2_beh; subst. inversion H4; subst.
+
+    eapply forward_simulation_same_safe_behavior.
+    + apply MultiSem.merged_prog_simulates_multisem; auto.
+    + eapply program_runs with (s:=(s,s0)).
+      * constructor; auto.
+        (* the states are mergeable *)
+        admit.
+      * eapply state_terminates with (s':=(s',s'0)); auto.
+        ** apply threeway_multisem_star.
+           *** (* the states are mergeable *) admit.
+           *** (* star in a bigger environment *) admit.
+           *** (* star in a bigger environment *) admit.
+        ** simpl. constructor; auto.
+    + simpl. constructor.
+  Admitted.
+
+  (* alternative without multisem *)
+
+  Theorem threeway_mt_star_simulation:
+    forall ips1 ips2 t ips1' ips2',
+      PS.mergeable_states (prog_interface prog2) (prog_interface prog1) ips1 ips2 ->
+      mt_star G (prog_interface prog2) ips1 t ips1' ->
+      mt_star G (prog_interface prog1) ips2 t ips2' ->
+      mt_star G empty_ctx (PS.merge_partial_states ips1 ips2) t
+                          (PS.merge_partial_states ips1' ips2').
+  Proof.
+  Admitted.
+
+  Theorem threeway_simulation_star:
+    forall ips1 ips2 t ips1' ips2',
+      PS.mergeable_states (prog_interface prog2) (prog_interface prog1) ips1 ips2 ->
+      star (PS.step (prog_interface prog2)) G ips1 t ips1' ->
+      star (PS.step (prog_interface prog1)) G ips2 t ips2' ->
+      star (PS.step empty_ctx) G (PS.merge_partial_states ips1 ips2) t
+                                 (PS.merge_partial_states ips1' ips2').
+  Proof.
+    intros ips1 ips2 t ips1' ips2'.
+    intros Hmergeable Hstar1 Hstar2.
+    apply star_mt_star_equivalence.
+    apply threeway_mt_star_simulation.
+    - assumption.
+    - apply star_mt_star_equivalence; assumption.
+    - apply star_mt_star_equivalence; assumption.
+  Qed.
+
+  Corollary partial_programs_composition':
+    forall t,
+      program_behaves (PS.sem prog1 (prog_interface prog2)) (Terminates t) ->
+      program_behaves (PS.sem prog2 (prog_interface prog1)) (Terminates t) ->
+      program_behaves (PS.sem prog empty_ctx) (Terminates t).
+  Proof.
+    intros t Hprog1_beh Hprog2_beh.
+    inversion Hprog1_beh; subst. inversion H0; subst.
+    inversion Hprog2_beh; subst. inversion H4; subst.
+
+    eapply program_runs with (s:=PS.merge_partial_states s s0).
+    - admit.
+    - eapply state_terminates with (s':=PS.merge_partial_states s' s'0); auto.
+      + apply threeway_simulation_star.
+        * admit.
+        * (* star in a bigger environment *) admit.
+        * (* star in a bigger environment *) admit.
+      + admit.
   Admitted.
 End PartialComposition.
 
@@ -379,15 +912,186 @@ Section Composition.
   Hypothesis closedness:
     closed_program (program_link p c mainC mainP).
 
-  Theorem composition:
-    forall beh,
-      program_behaves (PS.sem p (prog_interface c)) beh ->
-      program_behaves (PS.sem c (prog_interface p)) beh ->
-      program_behaves (CS.sem (program_link p c mainC mainP)) beh.
+  Theorem composition_for_termination:
+    forall t,
+      program_behaves (PS.sem p (prog_interface c)) (Terminates t) ->
+      program_behaves (PS.sem c (prog_interface p)) (Terminates t) ->
+      program_behaves (CS.sem (program_link p c mainC mainP)) (Terminates t).
   Proof.
-    intros beh Hbeh1 Hbeh2.
+    intros t Hbeh1 Hbeh2.
     destruct closedness.
-    eapply partial_semantics_implies_complete_semantics.
+    eapply partial_semantics_implies_complete_semantics; auto.
     apply partial_programs_composition; auto.
   Qed.
 End Composition.
+
+(*
+(* old stuff and thougths *)
+
+  (* not sure if this is useful, but it makes sense *)
+  Lemma step_after_merge_generic:
+    forall ips1 ips2,
+      PS.mergeable_states (prog_interface prog2) (prog_interface prog1) ips1 ips2 ->
+      (* the program is ips1 *)
+      (forall t ips1',
+         PS.step (prog_interface prog2) G ips1 t ips1' ->
+       exists ips2',
+         PS.mergeable_states (prog_interface prog2) (prog_interface prog1) ips1' ips2' /\
+         PS.step (prog_interface prog1) G ips2 t ips2' /\
+         PS.step empty_ctx G (PS.merge_partial_states ips1 ips2) t
+                             (PS.merge_partial_states ips1' ips2')) \/
+      (* the program is ips2 *)
+      (forall t ips2',
+         PS.step (prog_interface prog1) G ips2 t ips2' ->
+       exists ips1',
+         PS.mergeable_states (prog_interface prog2) (prog_interface prog1) ips1' ips2' /\
+         PS.step (prog_interface prog2) G ips1 t ips1' /\
+         PS.step empty_ctx G (PS.merge_partial_states ips1 ips2) t
+                             (PS.merge_partial_states ips1' ips2')).
+  Proof.
+  Admitted.
+
+  Lemma step_after_merge:
+    forall ips1 ips2 t ips1' ips2',
+      PS.step (prog_interface prog2) G ips1 t ips1' ->
+      PS.step (prog_interface prog1) G ips2 t ips2' ->
+      PS.mergeable_states (prog_interface prog2) (prog_interface prog1) ips1 ips2 ->
+      PS.step empty_ctx G (PS.merge_partial_states ips1 ips2) t
+                          (PS.merge_partial_states ips1' ips2') /\
+      PS.mergeable_states (prog_interface prog2) (prog_interface prog1) ips1' ips2'.
+  Proof.
+  Admitted.
+
+  Lemma decompose_visible_trace:
+    forall L s s' a t,
+      single_events L ->
+      Star L s (a::t) s' ->
+    exists s1 s2,
+      Star L s E0 s1 /\
+      Step L s1 [a] s2 /\
+      Star L s2 t s'.
+  Proof.
+  Admitted.
+
+  Lemma simulate_upto_visible_event:
+    forall ips1 ips2 a t ips1' ips2',
+      PS.mergeable_states (prog_interface prog2) (prog_interface prog1) ips1 ips2 ->
+      Star (PS.sem prog1 (prog_interface prog2)) ips1 (a::t) ips1' ->
+      Star (PS.sem prog2 (prog_interface prog1)) ips2 (a::t) ips2' ->
+    exists ips1'' ips2'',
+      (*Star (PS.sem prog1 (prog_interface prog2)) ips1 [a] ips1'' /\
+      Star (PS.sem prog2 (prog_interface prog1)) ips2 [a] ips2'' /\*)
+      PS.mergeable_states (prog_interface prog2) (prog_interface prog1) ips1'' ips2'' /\
+      Star (PS.sem prog empty_ctx) (PS.merge_partial_states ips1 ips2) [a]
+                                   (PS.merge_partial_states ips1'' ips2'') /\
+      Star (PS.sem prog1 (prog_interface prog2)) ips1'' t ips1' /\
+      Star (PS.sem prog2 (prog_interface prog1)) ips2'' t ips2'.
+  Proof.
+  Admitted.
+
+  (* merged states star given two partial star *)
+  Lemma star_after_merge:
+    forall ips1 ips2 t ips1' ips2',
+      PS.mergeable_states (prog_interface prog2) (prog_interface prog1) ips1 ips2 ->
+      Star (PS.sem prog1 (prog_interface prog2)) ips1 t ips1' ->
+      Star (PS.sem prog2 (prog_interface prog1)) ips2 t ips2' ->
+      PS.mergeable_states (prog_interface prog2) (prog_interface prog1) ips1' ips2' /\
+      Star (PS.sem prog empty_ctx) (PS.merge_partial_states ips1 ips2) t
+                                   (PS.merge_partial_states ips1' ips2').
+  Proof.
+    intros ips1 ips2 t ips1' ips2'.
+    intros Hmergeable Hstar1 Hstar2.
+
+    inversion Hmergeable; subst.
+
+    (* program has control in ips1 *)
+    - induction Hstar1; subst.
+      (* epsilon trace *)
+      + admit.
+      (* non-empty trace *)
+      + admit.
+
+    (* program has control in ips2 *)
+    - admit.
+
+  Admitted.
+
+  (*
+  Lemma sketch:
+    forall ips1 ips2 t ips1' ips2',
+      PS.mergeable_states (prog_interface prog2) (prog_interface prog1) ips1 ips2 ->
+      Star (PS.sem prog1 (prog_interface prog2)) ips1 t ips1' ->
+      Star (PS.sem prog2 (prog_interface prog1)) ips2 t ips2' ->
+      Star multisem (ips1, ips2) t (ips1', ips2').
+  Proof.
+    intros ips1 ips2 t ips1' ips2'.
+    intros Hmergeable Hstar1 Hstar2.
+    inversion Hmergeable; subst.
+    - induction Hstar1; subst.
+      + inversion Hstar2; subst.
+        * constructor.
+        * admit.
+      + inversion Hstar2; subst.
+        * symmetry in H6. apply Eapp_E0_inv in H6. destruct H6. subst.
+          exists s2.
+          exists (PS.CC (Pointer.component pc, pgps2, pmem2)).
+          apply star_step
+           with (t1:=E0) (t2:=E0)
+                (s2:=(s2, PS.CC (Pointer.component pc, pgps2, pmem2))).
+          ** unfold step. simpl. unfold G.
+             apply mstep.
+             *** unfold step in H1. simpl in *.
+                 (* this is our hypothesis, but with a bigger environment *) admit.
+             *** inversion H1; subst. simpl in *.
+                 apply PS.partial_step with ics ics'.
+                 **** (* this is our hypothesis, but with a bigger environment *) admit.
+                 **** do 2 CS.unfold_states.
+                      (* this should be true because of partialization *) admit.
+                 **** (* this should be true because of partialization *) admit.
+          ** econstructor.
+          ** reflexivity.
+        * (* we show that t1 = t0 because our semantics has single events,
+             then we use the inductive hypothesis *)
+          inversion H1; subst.
+          apply CS.singleton_traces in H7.
+          inversion H4; subst.
+          apply CS.singleton_traces in H10.
+          admit.
+    (* - symmetric to the first case *)
+  Admitted.
+       *)
+
+    (* since we truncate to prefixes, the following cases might not be needed *)
+
+    (*
+    (* silent divergence *)
+    - inversion H0; subst.
+      inversion H2; subst.
+      eapply forward_simulation_same_safe_behavior.
+      + apply prog_simulates_prog1_and_prog2.
+      + eapply program_runs with (s:=(s,s0)).
+        * constructor; auto.
+        * eapply state_diverges with (s':=(s',s'0)).
+          ** (* multisem simulates prog1 and prog2 *) admit.
+          ** econstructor; eauto.
+             *** admit.
+             *** admit.
+      + simpl. constructor.
+
+    (* reactive divergence *)
+    - inversion H0; subst.
+      inversion H2; subst.
+      eapply forward_simulation_same_safe_behavior.
+      + apply prog_simulates_prog1_and_prog2.
+      + eapply program_runs with (s:=(s,s0)).
+        * constructor; auto.
+        * eapply state_reacts.
+          ** (* multisem simulates prog1 and prog2 *) admit.
+      + simpl. constructor.
+
+    (* going wrong *)
+    - (* manually prove it *) admit.
+      *)
+  Admitted.
+
+*)
